Examples/ZX/VyZXInterface.v
@@ -1,2 +1,0 @@
-From TensorRocqEx Require Export ZXGraph VyZXTensor.
-From TensorRocq Require Export CospanHyperGraph.Semantics.
